Contour state gains importance

ContourStep.v
@@ -7,42 +7,36 @@ Require Import Trace.
 Require Import Machine.
 Require Import ObsTrace.
 
-(* This file covers a version of the trace properties in which the contour
-   is updated at each step. The contour can also remember the history of the
-   execution, carrying some arbitrary extra 
-   
-   First we define the annotation of a trace with contours given some contour
-   update function. *)
-Section WITH_CONTOUR_UPDATE.
+(* This file covers a version of the trace properties in which an arbitrary state
+   is carried alongside the machine state from which we will extrace a contour.*)
+Section WITH_CONTOUR_STATE.
 
   Variable ContourState : Type.
+  Variable ContourStateUpdate : MachineState -> ContourState -> ContourState.
 
-  Definition MCPState : Type := MachineState * Contour * PolicyState.
+  Definition MCPState : Type := MachineState * ContourState * PolicyState.
   Definition MCPTrace := TraceOf MCPState.
   Definition MPOTrace := MPTrace'.
 
-  Variable ContourStateUpdate : MachineState -> ContourState -> ContourState.
-  Variable OfState : ContourState -> Contour.
-
   (* WithContour relates an MPTrace to its MCPTrace given an initial contour state cs.
-     A finished trace (m,p) is related to (m,OfState c,p).
-     We relate a trace (notfinished (m,p) MP) to (notfinished (m,OfState c,p) MCP),
+     A finished trace (m,p) is related to (m,cs,p).
+     We relate a trace (notfinished (m,p) MP) to (notfinished (m,cs,p) MCP),
      where MP relates to MCP given cs' produced by ContourStateUpdate. Additionally,
      the relation requires that MP begin with m' and p' produced by mpstep (m,p),
      so that only MPTraces produced by the step function relate to any MCPTrace *)
   Inductive WithContour (cs:ContourState) : MPTrace -> MCPTrace -> Prop :=
   | WCFinished : forall m p,
-      WithContour cs (finished (m,p)) (finished (m,OfState cs,p))
+      WithContour cs (finished (m,p)) (finished (m,cs,p))
   | WCNotfinished : forall m p cs' m' p' o MP MCP,
       mpstep (m,p) = Some (m',p',o) ->
       ContourStateUpdate m cs = cs' ->
       WithContour cs' MP MCP ->
       head MP = (m',p') -> (* This checks that MP is actually real *)
-      WithContour cs (notfinished (m,p) MP) (notfinished (m,OfState cs,p) MCP).
+      WithContour cs (notfinished (m,p) MP) (notfinished (m,cs,p) MCP).
   
-  (* Similarly, we with WithObs turn an MCPTrace into the appropriate MPOTrace
-     with the observations of its steps. We always feed the observation produced
-     by a step forward, to line up with the machine state that follows that step. *)
+  (* Similarly, with WithObs we relate an MCPTrace into the MPOTrace
+     corresponding to its steps annotated with their observations. We feed
+     each step's observation forward, to line up with the machine state that follows that step. *)
   Inductive WithObs (o:Observation) : MCPTrace -> MPOTrace -> Prop :=
   | WOFinished : forall m c p,
       WithObs o (finished (m,c,p)) (finished (m,p,o))
@@ -56,101 +50,93 @@ Section WITH_CONTOUR_UPDATE.
      there is no observation until a step occurs. *)
   Definition ObsOfMCP := WithObs Tau.
 
-End WITH_CONTOUR_UPDATE.
+  (* ContourSegment relates two MCPTraces given a condition f on contour states, where the second
+     is a longest subtrace of the first such that f holds on all elements except the final.
+     So, it will always have at least two elements, and its head will be preceded by one
+     on which f does not hold, while the last (if any) also does not have f hold.
 
-(* ContourSegment relates two MCPTraces such that the first contains the second,
-   and the second is a longest subtrace subject to an initial and final condition, as follows.
-   
-   For MCP to relate to MCP' given conditions f1 and f2, f1 must hold on the head of MCP',
-   and f2 must not hold on any element of its tail except the final element if there is one.
-   (So f1 and f2 may both hold on the head of MCP', but if f2 holds on the next element MCP'
-   must be of length two.) Otherwise we take elements forever, or until we reach one on which
-   f2 holds.
+     We will use this machinery to clip out sections of a trace that fall under a particular
+     "domain", with the final state reflecting the state after that domain has finished.
+   *)
+  Inductive ContourSegment (f : ContourState -> Prop) : MCPTrace -> MCPTrace -> Prop :=
+  | CSCurrent : forall MCP MCP' m cs p,
+      head MCP = (m,cs,p) ->
+      f cs ->
+      PrefixUpTo (fun '(m,cs,p) => ~ f cs) MCP MCP' ->
+      ContourSegment f (notfinished (m,cs,p) MCP) (notfinished (m,cs,p) MCP')
+  | CSNot : forall MCP MCPpre MCPsuff MCP' m cs p,
+      head MCP = (m,cs,p) ->
+      ~ f cs ->
+      SplitInclusive (fun '(m,cs,p) => f cs) MCP MCPpre MCPsuff ->
+      ContourSegment f MCPsuff MCP' ->
+      ContourSegment f MCP MCP'
+  | CSSkip : forall MCP MCPpre MCPsuff MCP' m cs p,
+      head MCP = (m,cs,p) ->
+      f cs ->
+      SplitInclusive (fun '(m,cs,p) => f cs) MCP MCPpre MCPsuff ->
+      ContourSegment f MCPsuff MCP' ->
+      ContourSegment f MCP MCP'
+  .
 
-   f1 can be thought of as the condition that tells our property it needs to pay attention
-   to a subtrace, and f2 the condition that indicates that it needs to check whether something
-   has changed.
- *)
-Inductive ContourSegment (f1 f2 : Contour -> Prop) : MCPTrace -> MCPTrace -> Prop :=
-| CSCurrent : forall MCP MCP' m c p,
-    f1 c ->
-    PrefixUpTo (fun '(m,c,p) => f2 c) MCP MCP' ->
-    ContourSegment f1 f2 (notfinished (m,c,p) MCP) (notfinished (m,c,p) MCP')
-| CSNot : forall MCP MCPpre MCPsuff MCP' m c p,
-    head MCP = (m,c,p) ->
-    ~ f1 c ->
-    SplitInclusive (fun '(m,c,p) => f1 c) MCP MCPpre MCPsuff ->
-    ContourSegment f1 f2 MCPsuff MCP' ->
-    ContourSegment f1 f2 MCP MCP'
-| CSSkip : forall MCP MCPpre MCPsuff MCP' m c p,
-    head MCP = (m,c,p) ->
-    f1 c ->
-    SplitInclusive (fun '(m,c,p) => f2 c) MCP MCPpre MCPsuff ->
-    ContourSegment f1 f2 MCPsuff MCP' ->
-    ContourSegment f1 f2 MCP MCP'
-.
+  (* Moving on, we now discuss our trace properties, integrity and confidentiality.
+     These are properties of an MCPtrace and a component, intended to be applied to the subtraces
+     from ContourSegment - they treat the final state, if any, as a special end state
+     where they check what has changed over the course of the trace.
 
-(***** Integrity *****)
+     First, we need to check the contour of the subtrace, which is derived from
+     the contour state of its head, to see how the component should behave. So we
+     have a parameter of the map from contour states to contours. *)
 
-(* For integrity of a component k, we let f1 be the property that k is High Integrity *)
-Definition highInt (k:Component) := fun c => integrityOf (c k) = HI.
-(* And we let f2 be the property that k is either Low Integrity or Low Confidentiality *)
-Definition lowCI (k:Component) := fun c => confidentialityOf (c k) = LC \/ integrityOf (c k) = LI.
+  Variable ofContourState : ContourState -> Contour.
+  
+  (***** Integrity *****)
 
-(* The intuition is: if we see that a component is high integrity, we want to make sure that it
-   doesn't change until it is once again low integrity. We can check constantly, but if it is
-   high confidentiality, nothing should be reading it anyway; so it suffices to check that it is
-   unchanged only when it is low integrity or high [APT:low??] confidentiality, whichever comes first. *)
-(* APT: confidentiality part seems debateable.   Should integrity really depend on what is potentially readable rather than being based on observability? And if so, why should we check when integrity goes to LI if confidentiality never goes to LC? *)
+  (* First, we have ContourTraceIntegrity, which holds on a trace MCP and component k if
+     the first and last machine states agree on k. A segment that is infinite never breaks
+     integrity. *)
+  Definition ContourTraceIntegrity (MCP:MCPTrace) (k:Component) : Prop :=
+    forall m cs p m' cs' p',
+      integrityOf ((ofContourState cs) k) = HI ->
+      head MCP = (m,cs,p) ->
+      Last MCP (m',cs',p') ->
+      m k = m' k.
 
-(* APT: need an argument about why considering just a single component at a time captures right intuition. *)
+  (* Two machine states are variants at k if they agree on every component except k *)
+  (* APT: Fixed *)
+  Definition variantOf (k : Component) (m n : MachineState) :=
+    forall k', k <> k' -> m k' = n k'.
 
-(* Putting everything together, we have ContourTraceIntegrity, which holds on a trace if
-   for each component and every segment defined as above with regard to k, the first and
-   last machine states agree on k. A segment that is infinite never breaks integrity, because
-   k is never meant to be read again. *)
-Definition ContourTraceIntegrity (MCP:MCPTrace) : Prop :=
-  forall k MCP' m c p m' c' p',
-    ContourSegment (highInt k) (lowCI k) MCP MCP' ->
-    head MCP' = (m,c,p) ->
-    Last MCP' (m',c',p') ->
-    m k = m' k.
+  (* We can define a lazy version of trace integrity that does not check that k is
+     the same, but allows it to differ as long as it is never (APT: observably?) accessed.
+     The execution from the final state is compared to that of a run from any
+     k-variant, and the property holds if the protected execution is an
+     observational prefix of the variant. *)
+  Definition ContourTraceIntegrityLazy (MCP:MCPTrace) (k:Component) : Prop :=
+    forall m cs p m' cs' p',
+      integrityOf ((ofContourState cs) k) = HI ->
+      head MCP = (m,cs,p) ->
+      Last MCP (m',cs',p') ->
+      m k <> m' k ->  
+      forall m'', variantOf k m' m'' ->
+                  ObsOfMP (MPRunOf (m',p')) <=_O ObsOfM (RunOf  m'').
 
-(* Two machine states are variants at k if they agree on every component except k *)
-(* APT: Fixed *)
-Definition variantOf (k : Component) (m n : MachineState) :=
-  forall k', k <> k' -> m k' = n k'.
+  (* We might instead reset k to what it was initially. *)
+  Definition RollbackInt (k:Component) (Mstart Mend : MachineState) : MachineState :=
+    fun k0 => if keqb k k0 then Mstart k0 else Mend k0.
 
-(* We can define a lazy version of trace integrity that does not check that k is
-   the same, but allows it to differ as long as it is never (APT: observably?) accessed.
-   The execution from the final state is compared to that of a run from any
-   k-variant, and the property holds if the protected execution is an
-   observational prefix of the variant. *)
-Definition ContourTraceIntegrityLazy (MCP:MCPTrace) : Prop :=
-  forall k MCP' m c p m' c' p',
-    ContourSegment (highInt k) (lowCI k) MCP MCP' ->
-    head MCP' = (m,c,p) ->
-    Last MCP' (m',c',p') ->
-    m k <> m' k ->  
-    forall m'', variantOf k m' m'' ->
-                ObsOfMP (MPRunOf (m',p')) <=_O ObsOfM (RunOf  m'').
-
-(* We might instead reset k to what it was initially. *)
-(* APT: fixed *)
-Definition RollbackInt (k:Component) (Mstart Mend : MachineState) : MachineState :=
-  fun k0 => if keqb k k0 then Mstart k0 else Mend k0.
-
-(* This produces an even weaker property, in which it is permissible to
-   alter k (APT: even if it _is_ later accessed), as long as the remaining execution is not (APT observably) changed, perhaps
-   by coincidence. (APT: This needs clarification. *)
-Definition ContourTraceIntegrityLazier (MCP:MCPTrace) : Prop :=
-  forall k MCP' m c p m' c' p',
-    ContourSegment (highInt k) (lowCI k) MCP MCP' ->
-    head MCP' = (m,c,p) ->
-    Last MCP' (m',c',p') ->
+  (* This produces an even weaker property, in which it is permissible to
+     alter k and even to later access it, as long as the remaining execution 
+     is not observably changed. Such scenarios are easy to construct relative 
+     to a well-understood program, such as multiplying a value that is always
+     treated as a boolean by a nonzero constant, but are difficult to generalize. *)
+Definition ContourTraceIntegrityLazier (MCP:MCPTrace)  (k:Component) : Prop :=
+  forall m cs p m' cs' p',
+    integrityOf ((ofContourState cs) k) = HI ->
+    head MCP = (m,cs,p) ->
+    Last MCP (m',cs',p') ->
     ObsOfMP (MPRunOf (m',p')) <=_O ObsOfM (RunOf (RollbackInt k m m')).
 
-Lemma LazierWeaker : forall MCP, ContourTraceIntegrityLazy MCP -> ContourTraceIntegrityLazier MCP.
+Lemma LazierWeaker : forall MCP k, ContourTraceIntegrityLazy MCP k -> ContourTraceIntegrityLazier MCP k.
 Proof.
    unfold ContourTraceIntegrityLazy, ContourTraceIntegrityLazier.
    intros.
@@ -168,10 +154,6 @@ Qed.
 
 
 (***** Confidentiality *****)
-
-(* Our f1 and f2 conditions are now just that confidentiality is high, then low. *)
-Definition highConf (k:Component) := fun c => confidentialityOf (c k) = HC.
-Definition lowConf (k:Component) := fun c => confidentialityOf (c k) = LC.
 
 (* Intuitively, consider the #s to denote when a component is high confidentiality
    as execution moves across several security domains:
@@ -222,22 +204,22 @@ Definition Converge (m1 m2 : MachineState) :=
    - If the original trace gets stuck, then its observational trace should prefix that
      of the variant, which has no policy to get it stuck.
 *)
-Definition ContourTraceConfidentiality (MCP:MCPTrace) : Prop :=
-  forall k MCP' m c p m' MO MOv,
-    ContourSegment (highConf k) (lowConf k) MCP MCP' -> (* We consider all subtraces MCP' where any k is HC *)
-    head MCP' = (m,c,p) ->
-    ObsOfMCP MCP' MO -> (* We will mostly operate on the observation-annotated trace MCP' *)
+Definition ContourTraceConfidentiality (MCP:MCPTrace)  (k:Component) : Prop :=
+  forall m cs p m' MO MOv,
+    confidentialityOf ((ofContourState cs) k) = HC ->
+    head MCP = (m,cs,p) ->
+    ObsOfMCP MCP MO -> (* We will mostly operate on the observation-annotated trace MCP' *)
     variantOf k m m' -> (* We consider all states m' that are k-variants from m *)
-    RunOf m' = MOv -> (* And run m' to get an observation-annotated trace *)
+    PrefixUpTo (fun '(m',o) => Converge m m') (RunOf m') MOv ->
+    (* And run m' to get an observation-annotated trace *)
     (* These traces are related in their behavior. They either both converge, both diverge, or the
        original trace gets stuck (fail-stops).*)
-    (forall mend c p,
-        Last MCP' (mend,c,p) ->
-        confidentialityOf (c k) = LC -> (* if we actually get to low confidentiality *)
+    (forall mend p o,
+        Last MO (mend,p,o) ->
+        ~ Stuck MO ->
         exists m'converge o',
-          InTrace (m'converge, o') MOv /\ (* then the variant's trace will reach a state that converges *)
-          Converge mend m'converge /\
-          ObsOfMP MO ~=_O ObsOfM MOv /\ (* TODO: this needs to be the prefix *)
+          Last MOv (m'converge, o') /\ (* then the variant's trace will reach a state that converges *)
+          ObsOfMP MO ~=_O ObsOfM MOv /\
           (* both traces have the same observations *)
           deltaMatch m mend m' m'converge) /\ (* the converging states have changed identically *)
     (Infinite MO -> (* if the original trace is infinite, so is the variant, and their traces match *)
@@ -245,7 +227,7 @@ Definition ContourTraceConfidentiality (MCP:MCPTrace) : Prop :=
     (Stuck MO -> (* and if the original fail-stops, its trace is a prefix of that of the variant *)
      ObsOfMP MO <=_O ObsOfM MOv).
 (* APT: Didn't study carefully. *)
-
+End WITH_CONTOUR_STATE.
 
 (* In this section we will describe Domains, which describe the layout of code in our model.
    We will map components to domains as the ContourState, and that mapping may change during execution.
@@ -263,7 +245,7 @@ Section DomainTree.
   | shared
   | secret
   .
-
+  
   (* Our first actual domain is a Stack Domain. It has two forms: the active frame (everything above the
      stack pointer on entry) and a sealed stack (everything below). Of course a component that is in a
      sealed stack is also in some frame, and in fact may be in multiple nested sealed stacks.
@@ -271,7 +253,7 @@ Section DomainTree.
      In our actual properties, a component that is just in the active frame is always writeable;
      sharing determines how components are treated once they are at least one level down. *)
   Inductive StackD :=
-  | active : ShareStatus -> StackD
+  | active : ShareStatus -> option StackD -> StackD
   | sealed : StackD -> StackD
   .
 
@@ -312,7 +294,7 @@ Section WITH_MAPS.
         if isCode' cdm a
         then code
         else match findStack sm a with
-             | Some sid => stack sid (active secret)
+             | Some sid => stack sid (active secret None)
              | None => heap
              end
       | _ => registers
@@ -336,7 +318,7 @@ Section WITH_MAPS.
         | Mem a, stack sid sd =>
           if sidEq (Some sid) (findStack sm (m (Reg SP))) && wlt a (m (Reg SP))
           then stack sid (sealed sd)
-          else cs k
+          else stack sid (active secret (Some sd))
         | _,_ => cs k
         end
     | Some ret =>
@@ -346,19 +328,22 @@ Section WITH_MAPS.
           if sidEq (Some sid) (findStack sm (m (Reg SP))) then
             stack sid sd
           else cs k
+        | stack sid (active _ (Some sd)) =>
+          if sidEq (Some sid) (findStack sm (m (Reg SP))) then
+            stack sid sd
+          else cs k
         | _ => cs k
         end
     | Some (share k0) =>
       fun k =>
         if keqb k k0 then
           match cs k with
-          | stack sid (active secret) => stack sid (active shared)
+          | stack sid (active secret sd) => stack sid (active shared sd)
           | _ => cs k
           end
         else cs k
     | _ => cs
     end.
-
 
   (* Here's a very simple property: code is always low confidentiality and high integrity.
      So the contour maps code to (LC,HI), and everything else to (LC,LI) *)
@@ -369,13 +354,12 @@ Section WITH_MAPS.
       | _ => (LC,LI)
       end.
 
-  (* So our definition of CodeSafety is general safety instantiated with CodeInit and CodeUpdate *)
-  (* APT:???*)
   Definition CodeSafety :=
-    forall MCP,
-      WithContour ContourState updateCS CodeContour initCS (MPTraceOf mpInit) MCP ->
-      ContourTraceIntegrity MCP /\
-      ContourTraceConfidentiality MCP.    
+    forall MCP MCP' k ,
+      WithContour ContourState updateCS initCS (MPTraceOf mpInit) MCP ->
+      ContourSegment ContourState (fun cs => False) MCP MCP' ->
+      ContourTraceIntegrity ContourState CodeContour MCP k /\
+      ContourTraceConfidentiality ContourState CodeContour MCP k.    
 
   (* For coroutines, the active stack is accessible.
      All other stacks are inaccessible, and everything else is accessible.
@@ -393,19 +377,23 @@ Section WITH_MAPS.
       | _ => (LC, LI)
       end.
 
+  Definition InStack (d:Domain) (sid:StackID) : Prop :=
+    exists s,
+      d = stack sid s.
+
   Definition CoroutineSafety :=
-    forall MCP,
-      WithContour ContourState updateCS CoroutineContour initCS (MPTraceOf mpInit) MCP ->
-      ContourTraceIntegrity MCP /\
-      ContourTraceConfidentiality MCP.
-  
+    forall MCP sid k MCP',
+      WithContour ContourState updateCS initCS (MPTraceOf mpInit) MCP ->
+      ContourSegment ContourState (fun cs => ~ InStack (cs k) sid) MCP MCP' ->
+      ContourTraceIntegrity ContourState CoroutineContour MCP k /\
+      ContourTraceConfidentiality ContourState CoroutineContour MCP k.
 
   (* The subroutine property is a little more complicated. We will
      need to peel back nested stack domains to find whether a component has
      been shared. *)
   Fixpoint nestedStatus (sd:StackD) : ShareStatus :=
     match sd with
-    | active s => s
+    | active s _ => s
     | sealed sd => nestedStatus sd
     end.
 
@@ -418,7 +406,7 @@ Section WITH_MAPS.
   Definition SubroutineContour (cs:ContourState) : Contour :=
     fun k =>
       match cs k with
-      | stack sid (active secret) => (HC,LI)
+      | stack sid (active secret _) => (HC,LI)
       | stack sid sd =>
         match nestedStatus sd with
         | secret => (HC,HI)
@@ -426,11 +414,24 @@ Section WITH_MAPS.
         end
       | _ => (LC,LI)
       end.
-  
+
+  (* How do we split up functions? We don't! We check protection on a given stack component
+     from when it goes out of scope to when it returns. *)
+
   Definition StackSafety :=
-    forall MCP,
-      WithContour ContourState updateCS SubroutineContour initCS (MPTraceOf mpInit) MCP ->
-      ContourTraceIntegrity MCP /\
-      ContourTraceConfidentiality MCP.
+    forall MCP k sid sd MCP',
+      WithContour ContourState updateCS initCS (MPTraceOf mpInit) MCP ->
+      ContourSegment ContourState (fun cs => cs k = stack sid sd) MCP MCP' ->
+      ContourTraceIntegrity ContourState SubroutineContour MCP' k /\
+      ContourTraceConfidentiality ContourState SubroutineContour MCP' k.
+
+  (* APT: need an argument about why considering just a single component at a time captures right intuition. *)
+
+  (* In each of these properties, we've quantified over all components k and then checked
+     integrity and confidentiality of k specifically. We could imagine a version of, for instance,
+     confidentiality, where we vary multiple components simultaneously and see if that variation
+     changes behavior. Varying a single component is no stronger, because a variation where one
+     component is identical subsumes it. It is actually weaker: consider taking x || y, where
+     x and y are high confidentiality and initialized to 1. *)
 
 End WITH_MAPS.
